fix: transpose rt_closure for compatibility with ca

relations.v
@@ -15,7 +15,7 @@ Local Open Scope order_scope.
 Section well_founded.
 
 Definition sfrel {T : eqType} (f : T -> seq T) : rel T :=
-  [rel a b | b \in f a].
+  [rel a b | a \in f b].
 
 Definition filter_neq {T : eqType} (f : T -> seq T) : T -> seq T :=
   fun n => filter^~ (f n) (fun x => x != n).
@@ -31,7 +31,7 @@ Hypothesis descend : forall x n, x \in f n -> x <= n.
 Lemma filter_lt n k : k \in f\eq n -> k < n.
 Proof. by rewrite mem_filter lt_neqAle => /andP[] -> /descend ->. Qed.
 
-Lemma rel_sublt a b : (sfrel f\eq) a b -> b < a.
+Lemma rel_sublt a b : (sfrel f\eq) a b -> a < b.
 Proof. rewrite/sfrel /=. exact: filter_lt. Qed.
 
 (* Computation of the strict upward set of a given element
@@ -50,7 +50,7 @@ Equations(noind) s_up_set (n : T) : seq T by wf n (<%O : rel T) :=
     ys ++ ps.
 Next Obligation. exact: filter_lt. Qed.
 
-Definition t_closure (a b : T) : bool := b \in s_up_set a.
+Definition t_closure (a b : T) : bool := a \in s_up_set b.
 
 Lemma ext_s_up_set (x : T) (g h : forall y : T, y < x -> seq T) :
   (forall (y : T) (p : y < x), g y p = h y p) ->
@@ -61,10 +61,10 @@ Proof.
   congr flatten. apply/eq_in_map. move=> y /filter_lt. case: eqP=> //=.
 Qed.
 
-Lemma t_closure_lt a b : t_closure a b -> b < a.
+Lemma t_closure_lt a b : t_closure a b -> a < b.
 Proof.
   rewrite /t_closure.
-  move: a b. apply: wf_ind => a IH b.
+  move: b a. apply: wf_ind => a IH b.
   rewrite /s_up_set /Subterm.FixWf Fix_eq; last by apply: ext_s_up_set.
   rewrite {1}/s_up_set_functional mem_cat => /orP [/filter_lt //|].
   case/flatten_mapP=> x /filter_lt xinf.
@@ -72,27 +72,27 @@ Proof.
   by apply: lt_trans; first apply: ax.
 Qed.
 
-Lemma clos_trans_lt a b : clos_trans_n1 T (sfrel f\eq) a b -> b < a.
+Lemma clos_trans_lt a b : clos_trans_n1 T (sfrel f\eq) a b -> a < b.
 Proof.
   rewrite/sfrel /=.
   elim=> [x /filter_lt // | x y xfy acx ax].
-  apply: lt_trans; last by apply: ax.
+  apply: lt_trans; first by apply: ax.
   exact: filter_lt.
 Qed. 
 
 (* Transitive closure reflection lemma *)
 Lemma t_closureP a b : 
-  reflect (clos_trans_1n T (sfrel f\eq) a b) (t_closure a b).
+  reflect (clos_trans_n1 T (sfrel f\eq) a b) (t_closure a b).
 Proof.
   rewrite /t_closure.
-  move: a b. apply: wf_ind=> a IH b.
+  move: b a. apply: wf_ind=> a IH b.
   apply /(iffP idP).
   { rewrite /s_up_set /Subterm.FixWf Fix_eq; last by apply: ext_s_up_set.
     rewrite {1}/s_up_set_functional mem_cat => /orP [].
     { by constructor. }
     case/flatten_mapP=> x xinf. case: eqP=> //=.
     move=> /filter_lt /IH /apply H.
-    apply: Relation_Operators.t1n_trans; last exact H.
+    apply: Relation_Operators.tn1_trans; last exact: H.
     exact xinf. }
   move=> ctab. move: ctab IH. case.
   { rewrite /sfrel /= => c afc IH.
@@ -112,7 +112,7 @@ Qed.
  *)
 Definition up_set a := a :: s_up_set a.
 
-Definition rt_closure a b := b \in up_set a. 
+Definition rt_closure a b := a \in up_set b. 
 
 Lemma rt_closure_refl a : rt_closure a a.
 Proof. rewrite /rt_closure /up_set. exact: mem_head. Qed.
@@ -122,17 +122,17 @@ Lemma rt_closure_trans a b c :
 Proof.
   rewrite /rt_closure.
   rewrite !in_cons => /orP [/eqP -> //|].
-  move=> ba /orP [/eqP -> //|].
+  move=> ba /orP [/eqP <- //|].
   { by rewrite ba. }
   move=> cb. apply /orP. right.
-  apply /t_closureP. apply: clos_trans_t1n. apply: t_trans.
-  { apply /clos_t1n_trans /t_closureP. exact: ba. }
-  apply /clos_t1n_trans /t_closureP. exact: cb.
+  apply /t_closureP. apply: clos_trans_tn1. apply: t_trans.
+  { apply /clos_tn1_trans /t_closureP. exact: ba. }
+  apply /clos_tn1_trans /t_closureP. exact: cb.
 Qed.
 
 (* Reflexive-transitive closure reflection lemma *)
 Lemma rt_closureP a b :
-  reflect (clos_refl_trans_1n T (sfrel f) a b) (rt_closure a b).
+  reflect (clos_refl_trans_n1 T (sfrel f) a b) (rt_closure a b).
 Proof.
   apply /(iffP idP).
   { rewrite /rt_closure. 
@@ -140,25 +140,25 @@ Proof.
     { constructor. }
     move: (t_closureP a b). 
     rewrite /t_closure => refl. move: (refl atb). 
-    elim=> [c d cfd | c d e cfd st rt].
-    { apply: Relation_Operators.rt1n_trans; last by constructor.
+    elim => [ d cfd |  d e cfd st rt].
+    { apply: Relation_Operators.rtn1_trans; last by constructor.
       move: cfd. rewrite /sfrel /filter_neq //=.
       rewrite mem_filter. by move=> /andP [??]. }
-    apply: Relation_Operators.rt1n_trans; last exact: rt.
+    apply: Relation_Operators.rtn1_trans; last exact: rt.
     move: cfd. rewrite /sfrel /filter_neq //=.
     rewrite mem_filter. move=> /andP [? H]. exact: H. }
   move=> cab. rewrite /rt_closure /up_set.
   rewrite in_cons. apply/orP.
-  elim: cab => [| c d e st rt [/eqP -> | efd]]; first by left.
-  { case: (d =P c)=> [eq|neq] //=; first by left.
+  elim: cab => [|  d e st rt [/eqP -> | efd]]; first by left.
+  { case: (d =P e)=> [eq|neq] //=; first by left.
     right. move: st. rewrite /sfrel /=.
     rewrite /s_up_set /Subterm.FixWf Fix_eq; last by apply: ext_s_up_set.
     rewrite {1}/s_up_set_functional mem_cat /filter_neq mem_filter => ->.
      apply /orP. left. by apply /predD1P. }
-  case: (d =P c)=> [<-|neq] //=; first by right. 
-  right. move: (t_closureP d e)=> refl. move: (refl efd)=> ct.
-  apply /(t_closureP c e) /clos_trans_t1n /t_trans; first last.
-  { apply: clos_t1n_trans. exact: ct. }
+  case: (d =P e)=> [<-|neq] //=; first by right. 
+  right. move: (t_closureP a d)=> refl. move: (refl efd)=> ct.
+  apply /(t_closureP a e) /clos_trans_tn1 /t_trans.
+  { apply: clos_tn1_trans. exact: ct. }
   apply: t_step. rewrite /sfrel /filter_neq //=. 
   rewrite mem_filter. by apply /predD1P. 
 Qed.
